extended proofs for alternative ATC specs

FSM2.thy
@@ -33,6 +33,38 @@ lemma trace_alt_def: "trace r p = smap snd r" by (coinduction arbitrary: r p) (a
 definition language_state :: "('in, 'out, 'state) FSM \<Rightarrow> 'state \<Rightarrow> ('in \<times> 'out) list set" where
   "language_state M q \<equiv> {map fst r |r . path M r q}"
 
+lemma language_state_alt_def : "language_state M q = { io | io tr . path M  (io || tr) q \<and> length io = length tr }"
+proof -
+  have "language_state M q \<subseteq> { io | io tr . path M  (io || tr) q \<and> length io = length tr }"
+  proof 
+    fix xr assume xr_assm : "xr \<in> language_state M q"
+    then obtain r where r_def : "map fst r = xr" "path M r q" unfolding language_state_def by auto
+    then obtain xs ys where xr_split : "xr = xs || ys" "length xs = length ys" "length xs = length xr"
+      by (metis length_map zip_map_fst_snd) 
+    then have "(xs || ys) \<in> { io | io tr . path M  (io || tr) q \<and> length io = length tr }" using xr_assm r_def
+    proof -
+    have f1: "xs || ys = map fst r"
+      by (simp add: r_def(1) xr_split(1))
+      then have f2: "path M ((xs || ys) || take (min (length (xs || ys)) (length (map snd r))) (map snd r)) q"
+        by (simp add: r_def(2))
+      have "length (xs || ys) = length (take (min (length (xs || ys)) (length (map snd r))) (map snd r))"
+    using f1 by force
+      then show ?thesis
+        using f2 by blast
+    qed 
+    then show "xr \<in> { io | io tr . path M  (io || tr) q \<and> length io = length tr }" using xr_split by metis
+  qed
+  moreover have "{ io | io tr . path M  (io || tr) q \<and> length io = length tr } \<subseteq> language_state M q" 
+  proof 
+    fix xs assume xs_assm : "xs \<in> { io | io tr . path M  (io || tr) q \<and> length io = length tr }"
+    then obtain ys where ys_def : "path M (xs || ys) q" "length xs = length ys" by auto
+    then have "xs = map fst (xs || ys)" by auto
+    then show "xs \<in> language_state M q" using ys_def unfolding language_state_def by blast 
+  qed
+  ultimately show ?thesis by auto
+qed
+  
+
 lemma language_state[intro]:
   assumes "path M (w || r) q" "length w = length r"
   shows "w \<in> language_state M q"
@@ -102,34 +134,19 @@ lemma product_language_state[simp]: "language_state (product A B) (q1,q2) = lang
 
 
 
-definition finite_FSM :: "('in, 'out, 'state) FSM \<Rightarrow> bool" where
-  "finite_FSM M \<equiv> finite (nodes M)"
+fun finite_FSM :: "('in, 'out, 'state) FSM \<Rightarrow> bool" where
+  "finite_FSM M = finite (nodes M)"
 
-definition observable :: "('in, 'out, 'state) FSM \<Rightarrow> bool" where
-  "observable M \<equiv> \<forall> t . \<forall> s1 . ((succ M) t s1 = {}) \<or> (\<exists> s2 . (succ M) t s1 = {s2})"
+fun observable :: "('in, 'out, 'state) FSM \<Rightarrow> bool" where
+  "observable M = (\<forall> t . \<forall> s1 . ((succ M) t s1 = {}) \<or> (\<exists> s2 . (succ M) t s1 = {s2}))"
 
-definition completely_specified :: "('in, 'out, 'state) FSM \<Rightarrow> bool" where
-  "completely_specified M \<equiv> \<forall> s1 . \<forall> x \<in> inputs M . \<exists> y \<in> outputs M . \<exists> s2 . s2 \<in> (succ M) (x,y) s1"
+fun completely_specified :: "('in, 'out, 'state) FSM \<Rightarrow> bool" where
+  "completely_specified M = (\<forall> s1 . \<forall> x \<in> inputs M . \<exists> y \<in> outputs M . \<exists> s2 . s2 \<in> (succ M) (x,y) s1)"
 
-definition well_formed :: "('in, 'out, 'state) FSM \<Rightarrow> bool" where
-  "well_formed M \<equiv>
-    finite_FSM M
-    \<and> (\<forall> s1 x y . (x \<notin> inputs M \<or> y \<notin> outputs M) \<longrightarrow> succ M (x,y) s1 = {})"
-
-(*
-lemma observable_path_unique_singleton:
-  assumes "observable M"
-  and     "path M ([io] || [tr1]) q"
-  and     "path M ([io] || [tr2]) q"
-shows "tr1 = tr2"
-using assms unfolding observable_def
-proof -
-  assume "\<forall>t s1. succ M t s1 = {} \<or> (\<exists>s2. succ M t s1 = {s2})"
-  then show ?thesis
-    by (metis (no_types) FSM.path_cons_elim assms(2) assms(3) empty_iff prod.sel(1) prod.sel(2) singletonD zip_Cons_Cons)
-qed
-*)
-
+fun well_formed :: "('in, 'out, 'state) FSM \<Rightarrow> bool" where
+  "well_formed M =
+    (finite_FSM M
+    \<and> (\<forall> s1 x y . (x \<notin> inputs M \<or> y \<notin> outputs M) \<longrightarrow> succ M (x,y) s1 = {}))"
 
 
 lemma observable_path_unique[simp] :
@@ -153,7 +170,7 @@ proof (rule ccontr)
 
     have p1: "path M ([io_hd] || [tr1_hd]) q"   using Cons.prems tr_split by auto
     have p2: "path M ([io_hd] || [tr2_hd]) q"   using Cons.prems tr_split by auto
-    have tr_hd_eq : "tr1_hd = tr2_hd"           using Cons.prems unfolding observable_def
+    have tr_hd_eq : "tr1_hd = tr2_hd"           using Cons.prems unfolding observable.simps
      proof -
       assume "\<forall>t s1. succ M t s1 = {} \<or> (\<exists>s2. succ M t s1 = {s2})"
       then show ?thesis
@@ -166,7 +183,7 @@ proof (rule ccontr)
 qed
 
 
-lemma observable_path_unique_ex[elim] : 
+lemma observable_path_unique_ex : 
   assumes "observable M"
   and     "io \<in> language_state M q"
 obtains tr 
@@ -179,35 +196,218 @@ proof -
   ultimately show ?thesis using that by moura
 qed
 
+fun io_targets :: "('in, 'out, 'state) FSM \<Rightarrow> 'state \<Rightarrow> ('in \<times> 'out) list \<Rightarrow> 'state set" where
+  "io_targets M q io = { target (io || tr) q | tr . path M (io || tr) q \<and> length io = length tr }"
+
+lemma io_targets_observable_singleton_ex :
+  assumes "observable M"
+  and     "io \<in> language_state M q1"
+shows "\<exists> q2 . io_targets M q1 io = { q2 }"
+proof -
+  obtain tr where tr_def : "{ t . path M (io || t) q1 \<and> length io = length t } = { tr }" using assms observable_path_unique_ex by (metis (mono_tags, lifting)) 
+  then have "io_targets M q1 io = { target (io || tr) q1 }" by fastforce 
+  then show ?thesis by blast 
+qed
+
+lemma io_targets_observable_singleton_ob :
+  assumes "observable M"
+  and     "io \<in> language_state M q1"
+obtains q2 
+  where "io_targets M q1 io = { q2 }"
+proof -
+  obtain tr where tr_def : "{ t . path M (io || t) q1 \<and> length io = length t } = { tr }" using assms observable_path_unique_ex by (metis (mono_tags, lifting)) 
+  then have "io_targets M q1 io = { target (io || tr) q1 }" by fastforce 
+  then show ?thesis using that by blast 
+qed
 
 
-definition d_reachable :: "('in, 'out, 'state) FSM \<Rightarrow> 'state \<Rightarrow> 'state set" where
-  "d_reachable M p \<equiv> { q . (\<exists> xs ys tr . (path M ((xs || ys) || tr) p) \<and> target ((xs || ys) || tr) p = q 
-                             \<and> (\<forall> ys2 tr2 .  (path M ((xs || ys2) || tr2) p) \<longrightarrow> target ((xs || ys2) || tr2) p = q)) }"
+lemma io_targets_reachable :
+  assumes "q2 \<in> io_targets M q1 io"
+  shows "q2 \<in> reachable M q1" 
+  using assms  unfolding io_targets.simps by blast
+
+lemma io_targets_nodes :
+  assumes "q2 \<in> io_targets M q1 io"
+  and     "q1 \<in> nodes M"
+shows "q2 \<in> nodes M"
+  using assms by auto
+
+  
+
+fun d_reaches :: "('in, 'out, 'state) FSM \<Rightarrow> 'state \<Rightarrow> 'in list \<Rightarrow> 'state \<Rightarrow> bool" where
+  "d_reaches M p xs q = ((\<exists> ys tr . length xs = length ys \<and> length xs = length tr \<and> (path M ((xs || ys) || tr) p) \<and> target ((xs || ys) || tr) p = q) 
+                            \<and> (\<forall> ys2 tr2 .  (length xs = length ys2 \<and> length xs = length tr2 \<and> path M ((xs || ys2) || tr2) p) \<longrightarrow> target ((xs || ys2) || tr2) p = q))"
+
+lemma d_reaches_unique : 
+  assumes "d_reaches M p xs q1"
+  and    "d_reaches M p xs q2"
+shows "q1 = q2"
+using assms unfolding d_reaches.simps by blast
+
+lemma d_reaches_unique_cases : "{ q . d_reaches M (initial M) xs q } = {} \<or> (\<exists> q2 . { q . d_reaches M (initial M) xs q } = { q2 })"
+  unfolding d_reaches.simps by blast
+
+lemma d_reaches_unique_obtain[simp] :
+  assumes "d_reaches M (initial M) xs q"
+shows "{ p . d_reaches M (initial M) xs p } = { q }"
+  using assms unfolding d_reaches.simps by blast
+
+fun d_reachable :: "('in, 'out, 'state) FSM \<Rightarrow> 'state \<Rightarrow> 'state set" where
+  "d_reachable M p = { q . (\<exists> xs . d_reaches M p xs q) }"
 
 lemma d_reachable_reachable : "d_reachable M p \<subseteq> reachable M p" 
-proof -
-  have "d_reachable M p \<subseteq> {target r p |r. path M r p}"
+unfolding d_reaches.simps d_reachable.simps by blast
+
+fun is_det_state_cover_ass :: "('in, 'out, 'state) FSM \<Rightarrow> ('state \<Rightarrow> 'in list) \<Rightarrow> bool" where
+  "is_det_state_cover_ass M f = (\<forall> s \<in> d_reachable M (initial M) . d_reaches M (initial M) (f s) s)"
+
+lemma det_state_cover_ass_dist : 
+  assumes "is_det_state_cover_ass M f"
+  shows "\<forall> s1 \<in> d_reachable M (initial M) . \<forall> s2 \<in> d_reachable M (initial M) . s1 \<noteq> s2 \<longrightarrow> \<not>(d_reaches M (initial M) (f s2) s1)"
+  using assms unfolding d_reachable.simps is_det_state_cover_ass.simps 
   proof -
-    obtain aa :: "'a set \<Rightarrow> 'a set \<Rightarrow> 'a" where
-      f1: "\<forall>x0 x1. (\<exists>v2. v2 \<in> x1 \<and> v2 \<notin> x0) = (aa x0 x1 \<in> x1 \<and> aa x0 x1 \<notin> x0)"
-      by moura
-    { assume "\<exists>ps. aa {target ps p |ps. path M ps p} (d_reachable M p) = target ps p \<and> path M ps p"
-      then have "aa {target ps p |ps. path M ps p} (d_reachable M p) \<notin> d_reachable M p \<or> aa {target ps p |ps. path M ps p} (d_reachable M p) \<in> {target ps p |ps. path M ps p}"
-        by blast
-      then have ?thesis
-        using f1 by (meson subsetI) }
-    moreover
-    { assume "\<nexists>bs cs as. path M ((bs || cs) || as) p \<and> target ((bs || cs) || as) p = aa {target ps p |ps. path M ps p} (d_reachable M p) \<and> (\<forall>cs as. path M ((bs || cs) || as) p \<longrightarrow> target ((bs || cs) || as) p = aa {target ps p |ps. path M ps p} (d_reachable M p))"
-      then have "aa {target ps p |ps. path M ps p} (d_reachable M p) \<notin> d_reachable M p \<or> aa {target ps p |ps. path M ps p} (d_reachable M p) \<in> {target ps p |ps. path M ps p}"
-        by (simp add: d_reachable_def)
-      then have ?thesis
-        using f1 by (meson subsetI) }
-    ultimately show ?thesis
-      by metis
-  qed 
-  then show ?thesis by blast
+    assume "\<forall>s\<in>{q. \<exists>xs. d_reaches M (initial M) xs q}. d_reaches M (initial M) (f s) s"
+    then show "\<forall>c\<in>{c. \<exists>as. d_reaches M (initial M) as c}. \<forall>ca\<in>{c. \<exists>as. d_reaches M (initial M) as c}. c \<noteq> ca \<longrightarrow> \<not> d_reaches M (initial M) (f ca) c"
+      by (meson d_reaches_unique)
+  qed
+
+lemma det_state_cover_ass_diff :
+  assumes "is_det_state_cover_ass M f"
+  shows "\<forall> s1 \<in> d_reachable M (initial M) . \<forall> s2 \<in> d_reachable M (initial M) . s1 \<noteq> s2 \<longrightarrow> f s1 \<noteq> f s2"
+  using assms unfolding d_reachable.simps is_det_state_cover_ass.simps
+proof -
+  assume "\<forall>s\<in>{q. \<exists>xs. d_reaches M (initial M) xs q}. d_reaches M (initial M) (f s) s"
+  then show "\<forall>c\<in>{c. \<exists>as. d_reaches M (initial M) as c}. \<forall>ca\<in>{c. \<exists>as. d_reaches M (initial M) as c}. c \<noteq> ca \<longrightarrow> f c \<noteq> f ca"
+    by (metis (no_types) d_reaches_unique)
+qed 
+
+fun is_det_state_cover :: "('in, 'out, 'state) FSM \<Rightarrow> 'in list set \<Rightarrow> bool" where
+  "is_det_state_cover M V = (\<exists> f . is_det_state_cover_ass M f \<and> V = image f (d_reachable M (initial M)))"
+
+
+lemma det_state_cover_card :
+  assumes "is_det_state_cover M V"
+  and     "finite (nodes M)"
+shows   "card V = card (d_reachable M (initial M))"
+proof -
+  obtain f where f_def : "is_det_state_cover_ass M f \<and> V = image f (d_reachable M (initial M))"
+    using assms unfolding is_det_state_cover.simps by blast
+  then have card_f : "card V = card (image f (d_reachable M (initial M)))"
+    by simp
+
+  have "d_reachable M (initial M) \<subseteq> nodes M"
+    unfolding d_reachable.simps d_reaches.simps using d_reachable_reachable by blast
+  then have dr_finite : "finite (d_reachable M (initial M))"
+    using assms infinite_super by blast 
+
+  then have card_le : "card (image f (d_reachable M (initial M))) \<le> card (d_reachable M (initial M))"
+    using card_image_le by blast
+
+  have "card (image f (d_reachable M (initial M))) = card (d_reachable M (initial M))"
+    by (meson card_image det_state_cover_ass_diff f_def inj_onI)
+
+  then show ?thesis using card_f by auto
 qed
- 
+
+
+
+fun io_reduction :: "('in, 'out, 'state) FSM \<Rightarrow> ('in, 'out, 'state) FSM \<Rightarrow> bool" (infix "\<preceq>" 200)
+where "M1 \<preceq> M2 = (language_state M1 (initial M1) \<subseteq> language_state M2 (initial M2))"
+
+fun fault_model_m :: "('in, 'out, 'state) FSM \<Rightarrow> nat \<Rightarrow> (('in, 'out, 'state) FSM) set" where
+"fault_model_m M1 m = { M2 . 
+  well_formed M2 
+  \<and> inputs M1 = inputs M2 
+  \<and> outputs M1 = outputs M2
+  \<and> card (nodes M1) \<ge> m 
+  \<and> card (nodes M2) \<le> m 
+  \<and> observable M2 
+  \<and> completely_specified M2 }"
+
+
+
+lemma language_state_inclusion_next : 
+  assumes "language_state M1 q1 \<subseteq> language_state M2 q2"
+  and     "observable M1"
+  and     "observable M2"
+  and     "io_targets M1 q1 io = { q1t }"
+  and     "io_targets M2 q2 io = { q2t }"
+shows "language_state M1 q1t \<subseteq> language_state M2 q2t"
+using assms proof (induction io arbitrary: q1 q2)
+  case Nil
+  then show ?case by auto
+next
+  case (Cons io_hd io_tl)
+  then obtain x y where hs_split : "io_hd = (x,y)"  by (meson surj_pair)
+  then obtain tr where tr_def : 
+     "target (io_hd # io_tl || tr) q1 = q1t"
+     "path M1 (io_hd # io_tl || tr) q1" 
+     "length (io_hd # io_tl) = length tr" using Cons unfolding io_targets.simps
+  proof -
+    assume a1: "{target (io_hd # io_tl || tr) q1 |tr. path M1 (io_hd # io_tl || tr) q1 \<and> length (io_hd # io_tl) = length tr} = {q1t}"
+    assume a2: "\<And>tr. \<lbrakk>target (io_hd # io_tl || tr) q1 = q1t; path M1 (io_hd # io_tl || tr) q1; length (io_hd # io_tl) = length tr\<rbrakk> \<Longrightarrow> thesis"
+    have "\<exists>cs. q1t = target (io_hd # io_tl || cs) q1 \<and> path M1 (io_hd # io_tl || cs) q1 \<and> length (io_hd # io_tl) = length cs"
+      using a1 by blast
+    then show ?thesis using a2 by blast
+  qed 
+  then obtain q1x tr_tl where tr_split : "tr = q1x # tr_tl" by (metis Suc_length_conv)
+
+  then have "{t. path M1 (io_tl || t) q1x \<and> length io_tl = length t} = {tr_tl}" using observable_path_unique tr_def Cons.prems(2)
+    by (smt Collect_cong FSM.path_cons_elim language_state length_Cons nat.simps(1) singleton_conv snd_conv zip_Cons_Cons)    
+  moreover have 
+     "target (io_tl || tr_tl) q1x = q1t"
+     "path M1 (io_tl || tr_tl) q1x" 
+     "length io_tl = length tr_tl" using Cons tr_def tr_split unfolding io_targets.simps by auto
+  ultimately have tgt1 : "io_targets M1 q1x io_tl = { q1t }" using Cons.prems tr_def unfolding io_targets.simps  by auto
+
+  have "io_hd # io_tl \<in> language_state M2 q2" using Cons using tr_def(2) tr_def(3) by blast 
+  then obtain tr2 where tr2_def : 
+     "target (io_hd # io_tl || tr2) q2 = q2t"
+     "path M2 (io_hd # io_tl || tr2) q2" 
+     "length (io_hd # io_tl) = length tr2" using Cons unfolding io_targets.simps language_state_def
+  proof -
+    assume "{target (io_hd # io_tl || tr) q1 |tr. path M1 (io_hd # io_tl || tr) q1 \<and> length (io_hd # io_tl) = length tr} = {q1t}"
+    assume a1: "{target (io_hd # io_tl || tr) q2 |tr. path M2 (io_hd # io_tl || tr) q2 \<and> length (io_hd # io_tl) = length tr} = {q2t}"
+    assume a2: "\<And>tr2. \<lbrakk>target (io_hd # io_tl || tr2) q2 = q2t; path M2 (io_hd # io_tl || tr2) q2; length (io_hd # io_tl) = length tr2\<rbrakk> \<Longrightarrow> thesis"
+    have "\<exists>ds. q2t = target (io_hd # io_tl || ds) q2 \<and> path M2 (io_hd # io_tl || ds) q2 \<and> length (io_hd # io_tl) = length ds"
+      using a1 by blast
+    then show ?thesis using a2 by blast
+  qed 
+  then obtain q2x tr2_tl where tr2_split : "tr2 = q2x # tr2_tl" by (metis Suc_length_conv)
+
+  then have "{t. path M2 (io_tl || t) q2x \<and> length io_tl = length t} = {tr2_tl}"
+    by (smt Collect_cong FSM.path_cons_elim assms(3) language_state length_Cons nat.simps(1) observable_path_unique singleton_conv snd_conv tr2_def(2) tr2_def(3) zip_Cons_Cons) 
+  moreover have 
+     "target (io_tl || tr2_tl) q2x = q2t"
+     "path M2 (io_tl || tr2_tl) q2x" 
+     "length io_tl = length tr2_tl" using Cons tr2_def tr2_split unfolding io_targets.simps by auto
+  ultimately have tgt2 : "io_targets M2 q2x io_tl = { q2t }" using Cons.prems tr_def unfolding io_targets.simps  by auto
+
+  have "language_state M1 q1x \<subseteq> language_state M2 q2x" 
+  proof 
+    fix ioX assume ioX_assm : "ioX \<in> language_state M1 q1x"
+    then obtain tr1X where tr1X_def : "path M1 (ioX || tr1X) q1x" "length tr1X = length ioX" by auto
+    moreover have "path M1 [(io_hd,q1x)] q1" using tr_def tr_split Cons by auto
+    ultimately have "path M1 ((io_hd#ioX)|| (q1x#tr1X)) q1" "length (io_hd#ioX) = length (q1x#tr1X)" using tr1X_def by auto
+    then have "io_hd # ioX \<in> language_state M1 q1" by (metis language_state)
+    then have "io_hd # ioX \<in> language_state M2 q2" using Cons.prems by auto
+    then obtain q2x' tr2X where tr2X_def : "path M2 (io_hd # ioX || q2x' # tr2X) q2" "length tr2X = length ioX" by (metis language_state_elim length_Suc_conv) 
+
+    have "path M2 ([io_hd] || [q2x]) q2" using tr2_def(2) tr2_split by auto 
+    moreover have "path M2 ([io_hd] || [q2x']) q2" using tr2X_def(1) by auto 
+    moreover have "[io_hd] \<in> language_state M2 q2" using tr2X_def unfolding language_state_def
+    proof -
+      have "\<exists>ps. [io_hd] = map fst ps \<and> path M2 ps q2"
+        by (metis (no_types) calculation(2) list.size(3) list.size(4) map_fst_zip)
+      then show "[io_hd] \<in> {map fst ps |ps. path M2 ps q2}"
+        by blast
+    qed
+    ultimately have "q2x = q2x'" using observable_path_unique Cons.prems by (metis length_Cons list.inject list.size(3)) 
+
+    then show  "ioX \<in> language_state M2 q2x" using tr2X_def(1) tr2X_def(2) by auto 
+  qed
+
+  then show ?thesis using Cons.prems tgt1 tgt2 Cons.IH by auto
+qed
 
 end
